src/StcToObc/StcMemoryCorres.v
@@ -29,7 +29,7 @@ Module Type STCMEMORYCORRES
   Definition state_corres (s: ident) (S: state) (me: menv) : Prop :=
     find_inst s S ⌈≋⌉ find_inst s me.
 
-  Definition Memory_Corres_tcs
+  Definition Memory_Corres
              (tcs: list trconstr)
              (S I S': state)
              (me: menv) : Prop :=
@@ -48,252 +48,250 @@ Module Type STCMEMORYCORRES
         (Step_in s tcs ->
          state_corres s S' me)).
 
-  Lemma Memory_Corres_tcs_Def:
-    forall x ck ce S I S' me tcs,
-      Memory_Corres_tcs tcs S I S' me ->
-      Memory_Corres_tcs (TcDef x ck ce :: tcs) S I S' me.
-  Proof.
-    intros * (Lasts & Insts); split; [split|split; [|split]].
-    - inversion_clear 1 as [?? Last|]; eauto.
-      + inv Last.
-      + apply Lasts; auto.
-    - intro NLast; apply Lasts.
-      intro; apply NLast; right; auto.
-    - intros (Nstep & Nrst).
-      apply Insts; split.
-      + intro; apply Nstep; right; auto.
-      + intro; apply Nrst; right; auto.
-    - intros (Nstep & Rst).
-      apply Insts; split.
-      + intro; apply Nstep; right; auto.
-      + inversion_clear Rst as [?? IsSt|]; auto.
+  Section Preservation.
+
+    Variables (tcs: list trconstr) (S I S': state) (me: menv).
+    Hypothesis MemCorres:  Memory_Corres tcs S I S' me.
+
+    Lemma Memory_Corres_Def:
+      forall x ck ce,
+        Memory_Corres (TcDef x ck ce :: tcs) S I S' me.
+    Proof.
+      destruct MemCorres as (Lasts & Insts); intros; split; [split|split; [|split]].
+      - inversion_clear 1 as [?? Last|]; eauto.
+        + inv Last.
+        + apply Lasts; auto.
+      - intro NLast; apply Lasts.
+        intro; apply NLast; right; auto.
+      - intros (Nstep & Nrst).
+        apply Insts; split.
+        + intro; apply Nstep; right; auto.
+        + intro; apply Nrst; right; auto.
+      - intros (Nstep & Rst).
+        apply Insts; split.
+        + intro; apply Nstep; right; auto.
+        + inversion_clear Rst as [?? IsSt|]; auto.
+          inv IsSt.
+      - intros Step.
+        apply Insts; inversion_clear Step as [?? IsSt|]; auto.
         inv IsSt.
-    - intros Step.
-      apply Insts; inversion_clear Step as [?? IsSt|]; auto.
-      inv IsSt.
-  Qed.
+    Qed.
 
-  Lemma Memory_Corres_tcs_Next_present:
-    forall x ck e S I S' me tcs c,
-      Memory_Corres_tcs tcs S I S' me ->
-      find_val x S' = Some c ->
-      Memory_Corres_tcs (TcNext x ck e :: tcs) S I S' (add_val x c me).
-  Proof.
-    intros * (Lasts & Insts); split; [split|split; [|split]].
-    - inversion_clear 1 as [?? Last|?? Last]; eauto; unfold value_corres.
-      + inv Last; rewrite find_val_gss; auto.
-      + intros.
-        destruct (ident_eq_dec x0 x).
-        * subst; rewrite find_val_gss; auto.
-        * rewrite find_val_gso; auto;
-            apply Lasts with (1 := Last); auto.
-    - intros NLast **; unfold value_corres.
-      assert (x0 <> x)
-        by (intro; subst; apply NLast; left; constructor).
-      assert ( ~ Is_last_in x0 tcs)
-        by (intro; apply NLast; right; auto).
-      rewrite find_val_gso; auto;
-        apply Lasts; auto.
-    - intros (Nstep & Nrst).
-      assert (~ Step_in s tcs) by (intro; apply Nstep; right; auto).
-      assert (~ Reset_in s tcs) by (intro; apply Nrst; right; auto).
-      unfold state_corres; setoid_rewrite find_inst_add_val;
-        apply Insts; auto.
-    - intros (Nstep & Rst).
-      assert (~ Step_in s tcs) by (intro; apply Nstep; right; auto).
-      assert (Reset_in s tcs)
-        by (inversion_clear Rst as [?? IsSt|]; auto; inv IsSt).
-        apply Insts; auto.
-    - intros Step.
-      assert (Step_in s tcs)
-        by (inversion_clear Step as [?? IsSt|]; auto; inv IsSt).
-      unfold state_corres; setoid_rewrite find_inst_add_val;
-        apply Insts; auto.
-  Qed.
-
-  Lemma Memory_Corres_tcs_Next_absent:
-    forall x ck e S I S' me tcs,
-      Memory_Corres_tcs tcs S I S' me ->
-      find_val x S' = find_val x S ->
-      Memory_Corres_tcs (TcNext x ck e :: tcs) S I S' me.
-  Proof.
-    intros * (Lasts & Insts) Eq; split; [split|split; [|split]].
-    - inversion_clear 1 as [?? Last|?? Last]; eauto; unfold value_corres.
-      + inv Last.
-        destruct (Is_last_in_dec x tcs).
-        * apply Lasts; auto.
-        * setoid_rewrite Eq; apply Lasts; auto.
-      + apply Lasts; auto.
-    - intros NLast.
-      apply Lasts; intro; apply NLast; right; auto.
-    - intros (Nstep & Nrst).
-      apply Insts; split.
-      + intro; apply Nstep; right; auto.
-      + intro; apply Nrst; right; auto.
-    - intros (Nstep & Rst).
-      apply Insts; split.
-      + intro; apply Nstep; right; auto.
-      + inversion_clear Rst as [?? IsSt|]; auto.
-        inv IsSt.
-    - intros Step.
-      apply Insts; inversion_clear Step as [?? IsSt|]; auto.
-      inv IsSt.
-  Qed.
-
-  Lemma Memory_Corres_tcs_Reset_present:
-    forall s ck b S I S' Is me tcs me',
-      Memory_Corres_tcs tcs S I S' me ->
-      find_inst s I = Some Is ->
-      me' ≋ Is ->
-      ~ Step_in s tcs ->
-      Memory_Corres_tcs (TcReset s ck b :: tcs) S I S' (add_inst s me' me).
-  Proof.
-    intros * (Lasts & Insts) ? E; split; [split|split; [|split]].
-    - inversion_clear 1 as [?? Last|]; eauto.
-      + inv Last.
-      + apply Lasts; auto.
-    - intro NLast; apply Lasts.
-      intro; apply NLast; right; auto.
-    - intros (Nstep & Nrst).
-      assert (s0 <> s)
-        by (intro; subst; apply Nrst; left; constructor).
-      assert (~ Step_in s0 tcs) by (intro; apply Nstep; right; auto).
-      assert (~ Reset_in s0 tcs) by (intro; apply Nrst; right; auto).
-      unfold state_corres; rewrite find_inst_gso; auto;
-        apply Insts; auto.
-    - intros (Nstep & Rst).
-      unfold state_corres.
-      inversion_clear Rst as [?? Rst'|].
-      + inv Rst'.
-        setoid_rewrite find_inst_gss.
-        rewrite E; apply orel_eq_weaken; auto.
-      + destruct (ident_eq_dec s0 s).
-        * subst; rewrite find_inst_gss.
-          rewrite E; apply orel_eq_weaken; auto.
-        * assert (~ Step_in s0 tcs) by (intro; apply Nstep; right; auto).
-          rewrite find_inst_gso; auto;
-            apply (proj1 (proj2 (Insts s0))); auto.
-    - intros Step.
-      inversion_clear Step as [?? Step'|].
-      + inv Step'.
-      + unfold state_corres.
-        destruct (ident_eq_dec s0 s).
-        * subst; intuition.
-        * rewrite find_inst_gso; auto; apply Insts; auto.
-  Qed.
-
-  Lemma Memory_Corres_tcs_Reset_absent:
-    forall s ck b S I S' Is Ss me tcs,
-      Memory_Corres_tcs tcs S I S' me ->
-      find_inst s I = Some Is ->
-      find_inst s S = Some Ss ->
-      Is ≋ Ss ->
-      ~ Reset_in s tcs ->
-      Memory_Corres_tcs (TcReset s ck b :: tcs) S I S' me.
-  Proof.
-    intros * (Lasts & Insts) Find_I Find_S E; split; [split|split; [|split]].
-    - inversion_clear 1 as [?? Last|]; eauto.
-      + inv Last.
-      + apply Lasts; auto.
-    - intro NLast; apply Lasts.
-      intro; apply NLast; right; auto.
-    - intros (Nstep & Nrst).
-      apply Insts; split.
-      + intro; apply Nstep; right; auto.
-      + intro; apply Nrst; right; auto.
-    - intros (Nstep & Rst).
-      inversion_clear Rst as [?? Rst'|].
-      + inv Rst'.
+    Lemma Memory_Corres_Next_present:
+      forall x ck e c,
+        find_val x S' = Some c ->
+        Memory_Corres (TcNext x ck e :: tcs) S I S' (add_val x c me).
+    Proof.
+      destruct MemCorres as (Lasts & Insts); intros; split; [split|split; [|split]].
+      - inversion_clear 1 as [?? Last|?? Last]; eauto; unfold value_corres.
+        + inv Last; rewrite find_val_gss; auto.
+        + intros.
+          destruct (ident_eq_dec x0 x).
+          * subst; rewrite find_val_gss; auto.
+          * rewrite find_val_gso; auto;
+              apply Lasts with (1 := Last); auto.
+      - intros NLast **; unfold value_corres.
+        assert (x0 <> x)
+          by (intro; subst; apply NLast; left; constructor).
+        assert ( ~ Is_last_in x0 tcs)
+          by (intro; apply NLast; right; auto).
+        rewrite find_val_gso; auto;
+          apply Lasts; auto.
+      - intros (Nstep & Nrst).
         assert (~ Step_in s tcs) by (intro; apply Nstep; right; auto).
+        assert (~ Reset_in s tcs) by (intro; apply Nrst; right; auto).
+        unfold state_corres; setoid_rewrite find_inst_add_val;
+          apply Insts; auto.
+      - intros (Nstep & Rst).
+        assert (~ Step_in s tcs) by (intro; apply Nstep; right; auto).
+        assert (Reset_in s tcs)
+          by (inversion_clear Rst as [?? IsSt|]; auto; inv IsSt).
+        apply Insts; auto.
+      - intros Step.
+        assert (Step_in s tcs)
+          by (inversion_clear Step as [?? IsSt|]; auto; inv IsSt).
+        unfold state_corres; setoid_rewrite find_inst_add_val;
+          apply Insts; auto.
+    Qed.
+
+    Lemma Memory_Corres_Next_absent:
+      forall x ck e,
+        find_val x S' = find_val x S ->
+        Memory_Corres (TcNext x ck e :: tcs) S I S' me.
+    Proof.
+      destruct MemCorres as (Lasts & Insts); intros * Eq; split; [split|split; [|split]].
+      - inversion_clear 1 as [?? Last|?? Last]; eauto; unfold value_corres.
+        + inv Last.
+          destruct (Is_last_in_dec x tcs).
+          * apply Lasts; auto.
+          * setoid_rewrite Eq; apply Lasts; auto.
+        + apply Lasts; auto.
+      - intros NLast.
+        apply Lasts; intro; apply NLast; right; auto.
+      - intros (Nstep & Nrst).
+        apply Insts; split.
+        + intro; apply Nstep; right; auto.
+        + intro; apply Nrst; right; auto.
+      - intros (Nstep & Rst).
+        apply Insts; split.
+        + intro; apply Nstep; right; auto.
+        + inversion_clear Rst as [?? IsSt|]; auto.
+          inv IsSt.
+      - intros Step.
+        apply Insts; inversion_clear Step as [?? IsSt|]; auto.
+        inv IsSt.
+    Qed.
+
+    Lemma Memory_Corres_Reset_present:
+      forall s ck b Is me',
+        find_inst s I = Some Is ->
+        me' ≋ Is ->
+        ~ Step_in s tcs ->
+        Memory_Corres (TcReset s ck b :: tcs) S I S' (add_inst s me' me).
+    Proof.
+      destruct MemCorres as (Lasts & Insts); intros ?????? E; split; [split|split; [|split]].
+      - inversion_clear 1 as [?? Last|]; eauto.
+        + inv Last.
+        + apply Lasts; auto.
+      - intro NLast; apply Lasts.
+        intro; apply NLast; right; auto.
+      - intros (Nstep & Nrst).
+        assert (s0 <> s)
+          by (intro; subst; apply Nrst; left; constructor).
+        assert (~ Step_in s0 tcs) by (intro; apply Nstep; right; auto).
+        assert (~ Reset_in s0 tcs) by (intro; apply Nrst; right; auto).
+        unfold state_corres; rewrite find_inst_gso; auto;
+          apply Insts; auto.
+      - intros (Nstep & Rst).
         unfold state_corres.
-        rewrite Find_I, E, <-Find_S.
-        apply (proj1 (Insts s)); auto.
-      + apply Insts; split; auto.
-        intro; apply Nstep; right; auto.
-    - intros Step.
-      inversion_clear Step as [?? Step'|].
-      + inv Step'.
-      + apply Insts; eauto.
-  Qed.
-
-  Lemma Memory_Corres_tcs_Call_present:
-    forall s ys ck (rst: bool) b es S I S' Ss' tcs me me',
-      Memory_Corres_tcs tcs S I S' me ->
-      find_inst s S' = Some Ss' ->
-      me' ≋ Ss' ->
-      Memory_Corres_tcs (TcCall s ys ck rst b es :: tcs) S I S' (add_inst s me' me).
-  Proof.
-    intros * (Lasts & Insts) Find_S' E;
-      split; [split|split; [|split]].
-    - inversion_clear 1 as [?? Last|]; eauto.
-      + inv Last.
-      + apply Lasts; auto.
-    - intro NLast; apply Lasts.
-      intro; apply NLast; right; auto.
-    - intros (Nstep & Nrst).
-      assert (s0 <> s) as Neq
-          by (intro; subst; apply Nstep; left; constructor).
-      assert (~ Step_in s0 tcs) by (intro; apply Nstep; right; auto).
-      assert (~ Reset_in s0 tcs) by (intro; apply Nrst; right; auto).
-      unfold state_corres; rewrite find_inst_gso; auto;
-        apply Insts; auto.
-    - intros (Nstep & Rst).
-      assert (s0 <> s) as Neq
-          by (intro; subst; apply Nstep; left; constructor).
-      assert (~ Step_in s0 tcs) by (intro; apply Nstep; right; auto).
-      inversion_clear Rst as [?? Rst'|]; try inv Rst'.
-      unfold state_corres; rewrite find_inst_gso; auto;
-        apply Insts; auto.
-    - intros Step.
-      unfold state_corres.
-      inversion_clear Step as [?? Step'|].
-      + inv Step'.
-        rewrite find_inst_gss.
-        rewrite E; apply orel_eq_weaken; auto.
-      + destruct (ident_eq_dec s0 s).
-        * subst; rewrite find_inst_gss.
+        inversion_clear Rst as [?? Rst'|].
+        + inv Rst'.
+          setoid_rewrite find_inst_gss.
           rewrite E; apply orel_eq_weaken; auto.
-        * rewrite find_inst_gso; auto; apply Insts; auto.
-  Qed.
+        + destruct (ident_eq_dec s0 s).
+          * subst; rewrite find_inst_gss.
+            rewrite E; apply orel_eq_weaken; auto.
+          * assert (~ Step_in s0 tcs) by (intro; apply Nstep; right; auto).
+            rewrite find_inst_gso; auto;
+              apply (proj1 (proj2 (Insts s0))); auto.
+      - intros Step.
+        inversion_clear Step as [?? Step'|].
+        + inv Step'.
+        + unfold state_corres.
+          destruct (ident_eq_dec s0 s).
+          * subst; intuition.
+          * rewrite find_inst_gso; auto; apply Insts; auto.
+    Qed.
 
-  Lemma Memory_Corres_tcs_Call_absent:
-    forall s ys ck (rst: bool) b es S I S' Is Ss' tcs me,
-      Memory_Corres_tcs tcs S I S' me ->
-      find_inst s I = Some Is ->
-      (rst = false -> find_inst s S ⌈≋⌉ Some Is) ->
-      find_inst s S' = Some Ss' ->
-      Ss' ≋ Is ->
-      ~ Step_in s tcs /\ (if rst then Reset_in s tcs else ~ Reset_in s tcs) ->
-      Memory_Corres_tcs (TcCall s ys ck rst b es :: tcs) S I S' me.
-  Proof.
-    intros * (Lasts & Insts) Find_I Find_S Find_S' E NstepRst;
-      split; [split|split; [|split]].
-    - inversion_clear 1 as [?? Last|]; eauto.
-      + inv Last.
-      + apply Lasts; auto.
-    - intro NLast; apply Lasts.
-      intro; apply NLast; right; auto.
-    - intros (Nstep & Nrst).
-      apply Insts; split.
-      + intro; apply Nstep; right; auto.
-      + intro; apply Nrst; right; auto.
-    - intros (Nstep & Rst).
-      apply Insts; split.
-      + intro; apply Nstep; right; auto.
-      + inversion_clear Rst as [?? Rst'|]; auto.
-        inv Rst'.
-    - intros Step.
-      inversion_clear Step as [?? Step'|].
-      + inv Step'.
-        destruct rst; apply Insts in NstepRst.
-        * unfold state_corres in NstepRst; unfold state_corres.
-          rewrite <-NstepRst, Find_I, <-E.
-          apply orel_eq_weaken; auto.
-        * unfold state_corres in *.
-          rewrite <-NstepRst, Find_S, <-E; auto.
-          apply orel_eq_weaken; auto.
-      + apply Insts; eauto.
-  Qed.
+    Lemma Memory_Corres_Reset_absent:
+      forall s ck b Is Ss,
+        find_inst s I = Some Is ->
+        find_inst s S = Some Ss ->
+        Is ≋ Ss ->
+        ~ Reset_in s tcs ->
+        Memory_Corres (TcReset s ck b :: tcs) S I S' me.
+    Proof.
+      destruct MemCorres as (Lasts & Insts); intros ????? Find_I Find_S E; split; [split|split; [|split]].
+      - inversion_clear 1 as [?? Last|]; eauto.
+        + inv Last.
+        + apply Lasts; auto.
+      - intro NLast; apply Lasts.
+        intro; apply NLast; right; auto.
+      - intros (Nstep & Nrst).
+        apply Insts; split.
+        + intro; apply Nstep; right; auto.
+        + intro; apply Nrst; right; auto.
+      - intros (Nstep & Rst).
+        inversion_clear Rst as [?? Rst'|].
+        + inv Rst'.
+          assert (~ Step_in s tcs) by (intro; apply Nstep; right; auto).
+          unfold state_corres.
+          rewrite Find_I, E, <-Find_S.
+          apply (proj1 (Insts s)); auto.
+        + apply Insts; split; auto.
+          intro; apply Nstep; right; auto.
+      - intros Step.
+        inversion_clear Step as [?? Step'|].
+        + inv Step'.
+        + apply Insts; eauto.
+    Qed.
+
+    Lemma Memory_Corres_Call_present:
+      forall s ys ck (rst: bool) b es Ss' me',
+        find_inst s S' = Some Ss' ->
+        me' ≋ Ss' ->
+        Memory_Corres (TcCall s ys ck rst b es :: tcs) S I S' (add_inst s me' me).
+    Proof.
+      destruct MemCorres as (Lasts & Insts); intros ???????? Find_S' E;
+        split; [split|split; [|split]].
+      - inversion_clear 1 as [?? Last|]; eauto.
+        + inv Last.
+        + apply Lasts; auto.
+      - intro NLast; apply Lasts.
+        intro; apply NLast; right; auto.
+      - intros (Nstep & Nrst).
+        assert (s0 <> s) as Neq
+            by (intro; subst; apply Nstep; left; constructor).
+        assert (~ Step_in s0 tcs) by (intro; apply Nstep; right; auto).
+        assert (~ Reset_in s0 tcs) by (intro; apply Nrst; right; auto).
+        unfold state_corres; rewrite find_inst_gso; auto;
+          apply Insts; auto.
+      - intros (Nstep & Rst).
+        assert (s0 <> s) as Neq
+            by (intro; subst; apply Nstep; left; constructor).
+        assert (~ Step_in s0 tcs) by (intro; apply Nstep; right; auto).
+        inversion_clear Rst as [?? Rst'|]; try inv Rst'.
+        unfold state_corres; rewrite find_inst_gso; auto;
+          apply Insts; auto.
+      - intros Step.
+        unfold state_corres.
+        inversion_clear Step as [?? Step'|].
+        + inv Step'.
+          rewrite find_inst_gss.
+          rewrite E; apply orel_eq_weaken; auto.
+        + destruct (ident_eq_dec s0 s).
+          * subst; rewrite find_inst_gss.
+            rewrite E; apply orel_eq_weaken; auto.
+          * rewrite find_inst_gso; auto; apply Insts; auto.
+    Qed.
+
+    Lemma Memory_Corres_Call_absent:
+      forall s ys ck (rst: bool) b es Is Ss',
+        find_inst s I = Some Is ->
+        (rst = false -> find_inst s S ⌈≋⌉ Some Is) ->
+        find_inst s S' = Some Ss' ->
+        Ss' ≋ Is ->
+        ~ Step_in s tcs /\ (if rst then Reset_in s tcs else ~ Reset_in s tcs) ->
+        Memory_Corres (TcCall s ys ck rst b es :: tcs) S I S' me.
+    Proof.
+      destruct MemCorres as (Lasts & Insts); intros ???????? Find_I Find_S Find_S' E NstepRst;
+        split; [split|split; [|split]].
+      - inversion_clear 1 as [?? Last|]; eauto.
+        + inv Last.
+        + apply Lasts; auto.
+      - intro NLast; apply Lasts.
+        intro; apply NLast; right; auto.
+      - intros (Nstep & Nrst).
+        apply Insts; split.
+        + intro; apply Nstep; right; auto.
+        + intro; apply Nrst; right; auto.
+      - intros (Nstep & Rst).
+        apply Insts; split.
+        + intro; apply Nstep; right; auto.
+        + inversion_clear Rst as [?? Rst'|]; auto.
+          inv Rst'.
+      - intros Step.
+        inversion_clear Step as [?? Step'|].
+        + inv Step'.
+          destruct rst; apply Insts in NstepRst; unfold state_corres in *.
+          * rewrite <-NstepRst, Find_I, <-E.
+            apply orel_eq_weaken; auto.
+          * rewrite <-NstepRst, Find_S, <-E; auto.
+            apply orel_eq_weaken; auto.
+        + apply Insts; eauto.
+    Qed.
+
+  End Preservation.
 
 End STCMEMORYCORRES.
 
